pcuic/theories/PCUICInduction.v
@@ -37,7 +37,7 @@ Lemma term_forall_list_ind :
     (forall (s : projection) (t : term), P t -> P (tProj s t)) ->
     (forall (m : mfixpoint term) (n : nat), tFixProp P P m -> P (tFix m n)) ->
     (forall (m : mfixpoint term) (n : nat), tFixProp P P m -> P (tCoFix m n)) ->
-    (forall (i : Int63.int), P (tInt i)) ->
+    (* (forall (i : Int63.int), P (tInt i)) -> *)
 
     forall t : term, P t.
 Proof.
