template-coq/theories/Induction.v
@@ -37,7 +37,7 @@ Lemma term_forall_list_ind :
     (forall (s : projection) (t : term), P t -> P (tProj s t)) ->
     (forall (m : mfixpoint term) (n : nat), tFixProp P P m -> P (tFix m n)) ->
     (forall (m : mfixpoint term) (n : nat), tFixProp P P m -> P (tCoFix m n)) ->
-    (forall (i : Int63.int), P (tInt i)) ->
+    (* (forall (i : Int63.int), P (tInt i)) -> *)
     forall t : term, P t.
 Proof.
   intros until t. revert t.
@@ -96,7 +96,7 @@ Lemma term_wf_forall_list_ind :
     (forall (s : projection) (t : term), P t -> P (tProj s t)) ->
     (forall (m : mfixpoint term) (n : nat), tFixProp P P m -> Forall (fun def => isLambda (dbody def) = true) m -> P (tFix m n)) ->
     (forall (m : mfixpoint term) (n : nat), tFixProp P P m -> P (tCoFix m n)) ->
-    (forall (i : Int63.int), P (tInt i)) ->
+    (* (forall (i : Int63.int), P (tInt i)) -> *)
     forall t : term, wf t -> P t.
 Proof.
   intros until t. revert t.
@@ -114,19 +114,19 @@ Proof.
 
   apply H12; auto.
   red.
-  red in H19.
-  induction H19.
+  red in H18.
+  induction H18.
   constructor.
-  inv H23; auto.
+  inv H22; auto.
 
   apply H14. red.
-  red in H17.
-  induction H17. constructor.
-  inv H19; constructor; intuition auto.
-  clear H17; induction H19; constructor; intuition auto.
+  red in H16.
+  induction H16. constructor.
+  inv H18; constructor; intuition auto.
+  clear H16; induction H18; constructor; intuition auto.
 
   apply H15. red.
-  red in H17.
-  induction H17. constructor.
-  inv H19; constructor; intuition auto.
+  red in H16.
+  induction H16. constructor.
+  inv H18; constructor; intuition auto.
 Qed.
